proofs/itrees/it_exec.v
@@ -1,0 +1,190 @@
+From Coq Require Import
+     Arith.PeanoNat
+     Lists.List
+     Strings.String
+     Morphisms
+     Setoid
+     RelationClasses
+     EquivDec
+     Equality
+     Program.Tactics.
+
+From ExtLib Require Import
+     Data.String
+     Structures.Monad
+     Structures.Traversable
+     Data.List
+     Core.RelDec
+     Structures.Maps
+     Data.Map.FMapAList.
+
+From ITree Require Import
+     ITree
+     ITreeFacts
+     Monad
+     Basics.HeterogeneousRelations     
+     Events.Map
+     Events.State
+     Events.StateFacts
+     Events.Reader
+     Events.Exception
+     Events.FailFacts.
+
+Require Import Paco.paco.
+Require Import Psatz.
+Require Import ProofIrrelevance.
+Require Import FunctionalExtensionality.
+
+From mathcomp Require Import ssreflect ssrfun ssrbool ssrnat seq eqtype fintype.
+
+From ITree Require Import
+(*     Basics.Tacs *)
+     Basics.Category
+     Basics.Basics
+     Basics.Function
+     Core.ITreeDefinition
+     Core.KTree
+     Eq.Eqit
+     Eq.UpToTaus
+     Eq.Paco2
+     Indexed.Sum
+     Indexed.Function
+     Indexed.Relation
+     Interp.Handler
+     Interp.Interp
+     Interp.InterpFacts
+     Interp.Recursion.
+
+From ITree Require Import Rutt RuttFacts.
+
+From ITree Require Import EqAxiom.
+
+From Jasmin Require Import utils. (* expr psem_defs psem oseq. *)
+
+Import Monads.
+Import MonadNotation.
+Local Open Scope monad_scope.
+Local Open Scope option_scope.
+
+Obligation Tactic := done || idtac.
+
+(* This files contains the monad transformer associated with exec *)
+
+Variant result (E: Type) (A : Type) : Type :=
+    Ok of A | Error of E.
+
+Arguments Error {E} {A} s.
+Arguments Ok E [A] s.
+
+Definition exec t := result error t.
+
+
+
+Section ExecT.
+
+  Context {m : Type -> Type} {Fm: Functor.Functor m} {Mm : Monad m}
+    {MIm : MonadIter m}.
+
+  Definition execT (m : Type -> Type) (a : Type) : Type :=
+    m (exec a)%type.
+
+  Global Instance execT_fun : Functor.Functor (execT m) :=
+    {| Functor.fmap :=
+        fun X Y (f: X -> Y) => 
+          Functor.fmap (fun x =>
+                          match x with
+                          | Error e => Error e
+                          | Ok x => @Ok error Y (f x) end) |}.
+
+  Global Instance execT_monad : Monad (execT m) :=
+    {| ret := fun _ x => @ret m _ _ (Ok _ x);
+       bind := fun _ _ c k =>
+                 bind (m := m) c 
+                   (fun x => match x with
+                             | Error e => @ret m _ _ (Error e)
+                             | Ok x => k x end)
+    |}.
+
+  Global Instance execT_iter  : MonadIter (execT m) :=
+    fun A I body i => Basics.iter (M := m) (I := I) (R := exec A) 
+      (fun i => bind (m := m)
+               (body i)
+               (fun x => match x with
+                         | Error e       => ret (inr (Error e))
+                         | Ok (inl j) => @ret m _ _ (inl j)
+                         | Ok (inr a) => @ret m _ _ (inr (Ok _ a))
+                         end)) i.
+
+End ExecT.
+
+
+Section ExecTLaws. 
+
+Definition result_rel (W: Set) {X} (R : relation X) (Re : relation W) :
+   relation (result W X) :=
+fun (mx my : result W X) =>
+match mx with
+| Ok x => match my with
+            | Ok y => R x y
+            | Error _ => False
+            end
+| Error e0 => match my with
+          | Ok _ => False
+          | Error e1 => Re e0 e1 
+          end
+end.
+
+Definition exec_rel {X: Type} (R : relation X) :
+   relation (exec X) := result_rel error R (fun x y => True). 
+
+(* Universe inconsistency - and can't find a way to fix it *)
+(* Unset Universe Checking.  *)
+Global Instance execT_Eq1 {E} : Eq1 (execT (itree E)) :=
+  fun _ => eutt (exec_rel eq).
+
+Global Instance Reflexive_execT_eq1 {E T} : Reflexive (@execT_Eq1 E T).
+  Proof.
+    apply Reflexive_eqit.
+    intros []; reflexivity.
+Qed.
+
+Global Instance Symmetric_execT_eq1 {E T} : Symmetric (@execT_Eq1 E T).
+  Proof.
+    apply Symmetric_eqit.
+    unfold Symmetric.
+    intros [] [] H; auto; try reflexivity.
+    inv H; reflexivity.
+  Qed.
+
+Global Instance Transitive_execT_eq1 {E T} : Transitive (@execT_Eq1 E T).
+  Proof.
+    apply Transitive_eqit.
+    intros [] [] [] ? ?; subst; cbn in *; subst; intuition.
+  Qed.
+
+Global Instance Equivalence_execT_eq1 {E T} : Equivalence (@execT_Eq1 E T).
+  Proof.
+    split; typeclasses eauto.
+  Qed.
+
+Global Instance MonadLaws_execE {E} : MonadLawsE (execT (itree E)).
+  Proof.
+    split; cbn.
+    - cbn; intros; rewrite bind_ret_l; reflexivity.
+    - cbn; intros.
+      rewrite <- (bind_ret_r x) at 2.
+      eapply eutt_eq_bind; intros []; reflexivity.
+    - intros; cbn; rewrite bind_bind.
+      eapply eutt_eq_bind; intros []. 
+      + eapply eutt_eq_bind; intros []; reflexivity. 
+      + rewrite bind_ret_l; reflexivity.
+    - repeat intro; cbn.
+      eapply eutt_clo_bind; eauto.
+      intros [] [] REL; cbn in *; subst; try contradiction.
+      + apply H0.
+      + setoid_rewrite <- eutt_Ret. 
+        reflexivity.
+  Qed.
+  
+End ExecTLaws.
+
