proofs/itrees/it_jasmin_libF.v
@@ -1,0 +1,207 @@
+From Coq Require Import
+     Arith.PeanoNat
+     Lists.List
+     Strings.String
+     Morphisms
+     Setoid
+     RelationClasses
+     EquivDec
+     Equality
+     Program.Tactics.
+
+From ExtLib Require Import
+     Data.String
+     Structures.Monad
+     Structures.Traversable
+     Data.List
+     Core.RelDec
+     Structures.Maps
+     Data.Map.FMapAList.
+
+From ITree Require Import
+     ITree
+     ITreeFacts
+     Monad
+     Basics.HeterogeneousRelations     
+     Events.Map
+     Events.State
+     Events.StateFacts
+     Events.Reader
+     Events.Exception
+     Events.FailFacts.
+
+Require Import Paco.paco.
+Require Import Psatz.
+Require Import ProofIrrelevance.
+Require Import FunctionalExtensionality.
+
+From mathcomp Require Import ssreflect ssrfun ssrbool ssrnat seq eqtype fintype.
+
+From ITree Require Import
+(*     Basics.Tacs *)
+     Basics.Category
+     Basics.Basics
+     Basics.Function
+     Core.ITreeDefinition
+     Core.KTree
+     Eq.Eqit
+     Eq.UpToTaus
+     Eq.Paco2
+     Indexed.Sum
+     Indexed.Function
+     Indexed.Relation
+     Interp.Handler
+     Interp.Interp
+     Interp.InterpFacts
+     Interp.Recursion.
+
+From ITree Require Import Rutt RuttFacts.
+
+From ITree Require Import EqAxiom.
+
+From Jasmin Require Import utils. (*expr psem_defs psem oseq. *)
+
+Import Monads.
+Import MonadNotation.
+Local Open Scope monad_scope.
+Local Open Scope option_scope.
+
+Obligation Tactic := done || idtac.
+
+(* This files contains itrees general lemmas that depend on Jasmin
+files *)
+
+Section ExecT.
+
+  Context {m : Type -> Type} {Fm: Functor.Functor m} {Mm : Monad m}
+    {MIm : MonadIter m}.
+
+  Definition execT (m : Type -> Type) (a : Type) : Type :=
+    m (exec a)%type.
+
+  Global Instance execT_fun : Functor.Functor (execT m) :=
+    {| Functor.fmap :=
+        fun X Y (f: X -> Y) => 
+          Functor.fmap (fun x =>
+                          match x with
+                          | Error e => Error e
+                          | Ok x => @Ok error Y (f x) end) |}.
+
+  Global Instance execT_monad : Monad (execT m) :=
+    {| ret := fun _ x => @ret m _ _ (Ok _ x);
+       bind := fun _ _ c k =>
+                 bind (m := m) c 
+                   (fun x => match x with
+                             | Error e => @ret m _ _ (Error e)
+                             | Ok x => k x end)
+    |}.
+
+  Global Instance execT_iter  : MonadIter (execT m) :=
+    fun A I body i => Basics.iter (M := m) (I := I) (R := exec A) 
+      (fun i => bind (m := m)
+               (body i)
+               (fun x => match x with
+                         | Error e       => ret (inr (Error e))
+                         | Ok (inl j) => @ret m _ _ (inl j)
+                         | Ok (inr a) => @ret m _ _ (inr (Ok _ a))
+                         end)) i.
+
+End ExecT.
+
+
+Section ExecTLaws. 
+
+Definition result_rel (W: Set) {X} (R : relation X) (Re : relation W) :
+   relation (result W X) :=
+fun (mx my : result W X) =>
+match mx with
+| Ok x => match my with
+            | Ok y => R x y
+            | Error _ => False
+            end
+| Error e0 => match my with
+          | Ok _ => False
+          | Error e1 => Re e0 e1 
+          end
+end.
+
+Definition exec_rel {X: Type} (R : relation X) :
+   relation (exec X) := result_rel error R (fun x y => True). 
+
+Definition foo (X: Type) (ls: list X) : exec (list X) := Ok _ ls.
+
+From Jasmin Require Import var xseq type warray_ word. (*  psem_defs psem oseq. *)
+Require Import BinNums.
+
+
+Definition sem_t (t : stype) : Type :=
+  match t with
+  | sbool    => bool
+  | sint     => Z
+  | sarr n   => WArray.array n
+  | sword s  => unit (* Jasmin.word.word s *)
+  end.
+
+
+Definition sem_prod ts := (map sem_t ts).
+
+About lprod.
+Print lprod.
+Print map.
+
+Print WArray.array.
+
+(*
+Definition sem_ot (t:stype) : Type :=
+  if t is sbool then option bool
+  else sem_t t.
+
+Definition sem_tuple ts := ltuple (map sem_ot ts).
+
+Fixpoint sem_prod_ok {T: Type} (tin : seq stype) : sem_prod tin T -> sem_prod tin (exec T) :=
+  match tin return sem_prod tin T -> sem_prod tin (exec T) with
+  | [::] => fun o => ok o
+  | t :: ts => fun o v => @sem_prod_ok T ts (o v)
+  end.
+Arguments sem_prod_ok {T}%type_scope tin%seq_scope _.
+*)
+
+(* Universe inconsistency - and can't find a way to fix it *)
+(* Unset Universe Checking.  *)
+Fail Global Instance execT_Eq1 {E} : Eq1 (execT (itree E)) :=
+  fun _ => eutt (exec_rel eq).
+
+Set Printing Universes.
+
+About result.
+Print result.
+(*
+Variant
+result (E : Type@{result.u0}) (A : Type@{result.u1})
+  : Type@{max(Set,result.u0,result.u1)} :=
+    Ok : A -> result E A | Error : E -> result E A.
+
+Arguments result (E A)%type_scope
+Arguments Ok E%type_scope [A]%type_scope _
+Arguments Error {E A}%type_scope s
+  (where some original arguments have been renamed)
+ *)
+Check Ok.
+
+About Ok.
+Unset Printing Universes.
+
+Check Ok.
+
+Print exec.
+(*
+exec = [eta result error]
+     : Type@{exec.u0} -> Type@{max(Set,exec.u0)}
+
+Arguments exec t%type_scope
+*)
+
+End ExecTLaws.
+
+
+
