proofs/itrees/it_sems.v
@@ -60,7 +60,7 @@ From ITree Require Import Rutt RuttFacts.
 From ITree Require Import EqAxiom.
 
 From Jasmin Require Import expr psem_defs psem oseq.
-From Jasmin Require Import it_gen_lib it_jasmin_lib.
+From Jasmin Require Import it_gen_lib it_jasmin_lib it_exec.
 
 Import Monads.
 Import MonadNotation.
