proofs/itrees/it_with_analysis.v
@@ -1,0 +1,1096 @@
+From Coq Require Import
+     Arith.PeanoNat
+     Lists.List
+     Strings.String
+     Morphisms
+     Setoid
+     RelationClasses
+     EquivDec
+     Equality
+     Program.Tactics.
+
+From ExtLib Require Import
+     Data.String
+     Structures.Monad
+     Structures.Traversable
+     Data.List
+     Core.RelDec
+     Structures.Maps
+     Data.Map.FMapAList.
+
+From ITree Require Import
+     ITree
+     ITreeFacts
+     Monad
+     Basics.HeterogeneousRelations     
+     Events.Map
+     Events.State
+     Events.StateFacts
+     Events.Reader
+     Events.Exception
+     Events.FailFacts.
+
+Require Import Paco.paco.
+Require Import Psatz.
+Require Import ProofIrrelevance.
+Require Import FunctionalExtensionality.
+
+From mathcomp Require Import ssreflect ssrfun ssrbool ssrnat seq eqtype fintype.
+
+From ITree Require Import
+(*     Basics.Tacs *)
+     Basics.Category
+     Basics.Basics
+     Basics.Function
+     Core.ITreeDefinition
+     Core.KTree
+     Eq.Eqit
+     Eq.UpToTaus
+     Eq.Paco2
+     Indexed.Sum
+     Indexed.Function
+     Indexed.Relation
+     Interp.Handler
+     Interp.Interp
+     Interp.InterpFacts
+     Interp.Recursion.
+
+From ITree Require Import Rutt RuttFacts.
+
+From ITree Require Import EqAxiom.
+
+From Jasmin Require Import expr psem_defs psem oseq constant_prop
+                           constant_prop_proof.
+From Jasmin Require Import it_gen_lib it_jasmin_lib it_sems.
+
+Import Monads.
+Import MonadNotation.
+Local Open Scope monad_scope.
+Local Open Scope option_scope.
+
+(*
+Set Implicit Arguments.
+Unset Strict Implicit.
+Unset Printing Implicit Defensive.
+*)
+
+Obligation Tactic := done || idtac.
+
+(* PROBLEM with sections *)
+
+(* This files contains proofs to test the semantic models in
+ it_sems. It turns out that double recursion leads to a duplication of
+ inductive proofs, and thus that mutual recursion leads to simpler
+ proofs. The proofs on the modular model are still based on eutt and
+ need to be revised. The proofs on the flat models are much longer and
+ more laden with detail than those on the error-aware model. *)
+
+Section Lang.
+Context (asm_op: Type) (asmop: asmOp asm_op).
+
+Section WSW.
+Context {wsw: WithSubWord}.   
+Context
+  (dc: DirectCall)
+  (syscall_state : Type)
+  (ep : EstateParams syscall_state)
+  (spp : SemPexprParams)
+  (sip : SemInstrParams asm_op syscall_state)
+  (pT : progT)
+  (scP : semCallParams)
+  (ev : extra_val_t).
+
+Local Notation StackE := (StackE ep).
+Local Notation estack := (estack ep).
+Local Notation FunE := (FunE asmop).
+Local Notation InstrE := (InstrE asmop).
+Local Notation AssgnE := (AssgnE asmop).
+Local Notation WriteIndex := (WriteIndex asmop).
+Local Notation InitState := (InitState asmop).
+Local Notation SetDests := (SetDests asmop).
+Local Notation CState := (CState asmop).
+Local Notation FFCall_ := (FFCall asmop). 
+Local Notation PFCall_ := (PFCall asmop). 
+Local Notation cmd_Ind := (cmd_Ind asm_op asmop).
+Local Notation FunDef := (FunDef asmop pT).
+Local Notation FCState := (FCState asmop ep).
+Local Notation PCState := (PCState asmop ep).
+Local Notation meval_instr := (meval_instr spp scP). 
+Local Notation pmeval_instr := (pmeval_instr spp scP). 
+Local Notation peval_instr_call := (peval_instr_call dc spp scP). 
+Local Notation evalE_fun := (evalE_fun dc spp scP ev).
+Local Notation meval_fcall := (meval_fcall dc spp scP ev). 
+Local Notation mevalE_cmd := (mevalE_cmd dc spp scP ev). 
+Local Notation pmeval_cmd := (pmeval_cmd dc spp scP ev). 
+Local Notation peval_fcall_body := (peval_fcall_body dc spp scP ev). 
+Local Notation pmeval_fcall := (pmeval_fcall dc spp scP ev). 
+Local Notation peval_flat_cmd := (peval_flat_cmd dc spp scP ev). 
+Local Notation interp_InstrE := (interp_InstrE dc spp scP ev).
+
+
+(***************************************************************************)
+(*** APPLICATION ***********************************************************)
+(** we define a language translation and try to prove equivalence of
+function application and commands across the translation under the
+appropriate hypothesis. First we specify the translation. *)
+
+(*** TRANSLATION SPEC *******************************************)
+Section TRANSF.
+
+  Check Monad.
+  About Monad.
+  Check stateT.
+  About Monad.
+  About state.
+  About stateT.
+  Check fold_left.
+  About ITree.map.
+
+  Check fold_left.
+  About state.
+  
+(*  Lemma xxx {S} : Monad (state S).
+  auto.
+*)
+
+  (* useless without monad laws *)
+#[global] Instance Monad_state {s} : Monad (state s)
+  := {|
+    ret _ a := fun s => (s, a) ;
+    bind _ _ t k := fun s =>
+      let sa := t s in
+      k (snd sa) (fst sa)
+    |}.
+
+(*
+#[global] Instance Eq1_prod {s} : Eq1 (prod s).
+unfold Eq1.
+intro A.
+exact (eq).
+Defined.
+ *)
+
+Global Instance Monad_identity : Monad identity.
+  econstructor.
+  - intros T t. exact t.
+  - intros T U m f. exact (f m). 
+Defined.
+
+Global Instance Eq1_identity : Eq1 identity.
+Proof.
+  unfold Eq1.
+  intro A. exact eq.
+Defined.
+
+Global Instance Eq1Equivalence_identity :
+  @Eq1Equivalence identity _ Eq1_identity.
+Proof.
+  econstructor; simpl; repeat intuition.
+Qed.
+
+Definition stateM := fun S => stateT S identity.
+
+Fixpoint mapS {S A B} (f: A -> stateM S B) (ls: list A) (b: B) :
+  stateM S B :=
+  match ls with
+  | nil => ret b
+  | x :: xs => bind (f x) (mapS f xs) end.            
+
+(*
+Fixpoint mapL {S A B} (f: A -> stateM S B) (ls: list A) (s: S) :
+  (S * (list B)) :=
+  match ls with
+  | nil => ((ret nil) : stateM S (list B)) s
+  | x :: xs => (x' <- f x ;; xs' <- mapL f xs ;; ret (x' :: xs')) s end.        *)    
+
+Fixpoint mapL {S A B} (f: A -> stateM S B) (ls: list A) :
+  stateM S (list B) :=
+  match ls with
+  | nil => ret nil
+  | x :: xs => x' <- f x ;; xs' <- mapL f xs ;; ret (x' :: xs') end.            
+
+Context (I: Type).
+
+Context (tr_lval : lval -> stateM I lval)
+        (tr_expr : pexpr -> stateM I pexpr)
+        (tr_opn : sopn -> stateM I sopn)
+        (tr_sysc : syscall_t -> stateM I syscall_t).
+
+Local Notation tr_lvals ls := (mapL tr_lval ls).
+Local Notation tr_exprs es := (mapL tr_expr es).
+
+Definition Tr_i (Th: instr_r -> stateM I instr_r) (i: instr) :
+  stateM I instr :=
+  match i with MkI ii ir => ir' <- Th ir ;; ret (MkI ii ir') end.  
+
+Fixpoint Tr_ir (i : instr_r) : stateM I instr_r :=
+  let R := Tr_i Tr_ir in 
+  match i with
+  | Cassgn x tg ty e =>
+      x' <- tr_lval x ;; e' <- tr_expr e ;;
+      ret (Cassgn x' tg ty e')
+  | Copn xs tg o es =>
+      xs' <- tr_lvals xs ;;
+      o' <- tr_opn o ;;
+      es' <- tr_exprs es ;;
+      ret (Copn xs' tg o' es')
+  | Csyscall xs sc es =>
+      xs' <- tr_lvals xs ;;
+      sc' <- tr_sysc sc ;;
+      es' <- tr_exprs es ;;
+      ret (Csyscall xs' sc' es')
+  | Cif e c1 c2 => 
+      e' <- tr_expr e ;;
+      c1' <- mapL R c1 ;;
+      c2' <- mapL R c2 ;;
+      ret (Cif e' c1' c2') 
+  | Cfor i rg c =>
+      c' <- mapL R c ;;
+      ret (Cfor i rg c')                     
+  | Cwhile a c1 e c2 =>
+      c1' <- mapL R c1 ;;
+      e' <- tr_expr e ;;
+      c2' <- mapL R c2 ;;
+      ret (Cwhile a c1' e' c2')
+  | Ccall xs fn es =>
+      xs' <- tr_lvals xs ;;
+      es' <- tr_exprs es ;;
+      ret (Ccall xs' fn es')
+  end.
+Local Notation Tr_instr := (Tr_i Tr_ir).
+Local Notation Tr_cmd c := (mapL Tr_instr c).
+
+Definition Tr_FunDef (f: FunDef) : stateM I FunDef :=
+  match f with
+  | MkFun i tyin p_xs c tyout r_xs xtr =>
+    c' <- Tr_cmd c ;;  
+    ret (MkFun i tyin p_xs c' tyout r_xs xtr) end.
+
+(*
+
+We would like to support undefined behaviour, CompCert-style, thus relating by a relation such as eutt or rutt source programs that go wrong with compiled ones that can behave arbitrarily after a source error is thrown.
+
+Of course it is possible to relate 'throw Error' with any visible event, and by interpreting 'Throw' with e.g.
+
+    Definition handle_Err {E} : exceptE Err ~> failT (itree E) :=  fun _ _ => Ret (None).
+
+we could also relate it to any returned value. 
+
+But correct me if I'm wrong, if the compiled program diverges, we would need a further clause in the relation, specifically allowing for 'throw' to be related with a tau transition. 
+ 
+I was wondering if this problem has already been handled anywhere, either in this or other ways. 
+
+Lemma ggg {S A} : True -> failT (stateT S identity) A.  
+  unfold failT, stateT; simpl.  Abort.
+
+Lemma ggg {S A} : True -> execT (stateT S identity) A.  
+  unfold execT; simpl.  Abort.
+
+Print exec.
+Print result.
+
+Lemma ggg {S A} : True -> (stateT S identity) (exec A).  
+  unfold exec; simpl.  Abort.
+
+Print exec.
+Print result.
+
+Lemma ggg {S A} : stateT S identity (exec A).  
+  unfold execT; simpl.  Abort.
+
+Lemma ggg {S A} : stateT S (failT identity) A.  
+  unfold execT; simpl.  Abort.
+
+Check option.
+Check result.
+
+Check error.
+Print error.
+Check @Ok.
+Check result.
+Print exec.
+Check execT.
+Check failT.
+
+Set Universe Polymorphism.
+
+Definition execTT (m : Type -> Type) (a : Type) : Type :=
+    m (result error a).
+
+Definition failTT (m : Type -> Type) (a : Type) : Type :=
+    m (option a).
+
+Definition execI : Type -> Type := execTT identity.
+
+Definition failI : Type -> Type := failTT identity.
+
+Definition execP {E} (m : Type -> Type) (a : Type) : Type :=
+    m (result E a).
+
+Definition execI' {E} : Type -> Type := @execP E identity.
+
+About stateT.
+
+Check StateMonad.stateT.
+
+About StateMonad.stateT.
+
+
+Lemma ggg (S A: Type) : True -> stateT S (failT identity) A.  
+  unfold failT; simpl. unfold identity; simpl.
+  unfold stateT. Abort.
+
+Lemma ggg (S A: Type) : True -> stateT S identity (option A).  
+  unfold stateT; simpl. unfold identity; simpl. Abort.
+
+Lemma ggg (S A: Type) : True -> S -> exec (S * A).  
+  unfold stateT; simpl. unfold identity; simpl.
+
+  Print Iter.
+  Print Iterative.
+  Print MonadIter.
+*)
+  
+(* 
+
+NEED TO PROVE MORE STUFF ABOUT execT - see FailFacts.v 
+(especially MonadLaws_failE).
+
+*)
+
+  
+  
+(*********************************************************************)
+(*** PROOFS **********************************************************)
+
+(*
+Section GEN_ErrAndFlat.
+
+Context (E: Type -> Type).   
+
+Local Notation RV := (PR values).
+Local Notation VS := (values * estate)%type.
+Local Notation FVS := (funname * VS)%type.
+
+Notation RVS := (fun (vs_st1 vs_st2 : VS) => 
+  (RV vs_st1.1 vs_st2.1 /\ RS vs_st1.2 vs_st2.2)).
+Notation RFVS := (fun (fvs1 fvs2 : FVS) => 
+  (fvs1.1 = fvs2.1 /\ RVS fvs1.2 fvs2.2)).
+Notation RC := (fun c1 c2: cmd => c2 = Tr_cmd c1).
+Notation RFunDef := (fun f1 f2: FunDef => f2 = Tr_FunDef f1).
+
+Context (rvs_def : PR VS = RVS)
+        (rfvs_def : PR FVS = RFVS)
+        (rc_def : PR cmd = RC)
+        (rfundef_def : PR FunDef = RFunDef).
+*)
+
+Section Sample_proof.
+
+Context (E: Type -> Type).   
+Context (HasErr: ErrState -< E).   
+
+Context (pr1 pr2 : prog)
+        (PR : forall T, T -> T -> Prop).
+Context (TR_E : forall (E: Type -> Type) T1 T2,
+            E T1 -> E T2 -> Prop)
+        (VR_E : forall (E: Type -> Type) T1 T2,
+            E T1 -> T1 -> E T2 -> T2 -> Prop).
+
+Local Notation RS := (PR estate).
+Local Notation RV := (PR values).
+Local Notation RV1 := (PR value).
+(* Local Notation RSMV := (PR (syscall_state * mem * seq value)). *)
+
+Local Notation VS := (values * estate)%type.
+Local Notation FVS := (funname * VS)%type.
+
+Notation RVS := (fun (vs_st1 vs_st2 : VS) => 
+  (RV vs_st1.1 vs_st2.1 /\ RS vs_st1.2 vs_st2.2)).
+Notation RFVS := (fun (fvs1 fvs2 : FVS) => 
+  (fvs1.1 = fvs2.1 /\ RVS fvs1.2 fvs2.2)).
+Notation RC := (fun c1 c2: cmd => c2 = Tr_cmd c1).
+Notation RFunDef := (fun f1 f2: FunDef => f2 = Tr_FunDef f1).
+
+Context (rvs_def : PR VS = RVS)
+        (rfvs_def : PR FVS = RFVS)
+        (rc_def : PR cmd = RC)
+        (rfundef_def : PR FunDef = RFunDef).
+
+(*
+(* DE: relation between call events, i.e. over inputs of type 
+# (funname * (values * estate)) *)
+Definition TR_D_DE {T1 T2} (d1 : callE FVS VS T1)
+                           (d2 : callE FVS VS T2) : Prop :=
+  match (d1, d2) with
+  | (Call f1, Call f2) => RFVS f1 f2 end.               
+
+(* DE: relation between call outputs, i.e. (values * estate) *)
+Program Definition VR_D_DE {T1 T2} (d1 : callE FVS VS T1) (t1: T1)
+                                 (d2 : callE FVS VS T2) (t2: T2) : Prop.
+  dependent destruction d1.
+  dependent destruction d2.
+  exact (RVS t1 t2).
+Defined.
+
+Lemma comp_gen_ok_DE (fn: funname) (vs1 vs2: values) (st1 st2: estate) :
+  RV vs1 vs2 ->
+  RS st1 st2 ->
+  @rutt (callE FVS VS +' E) (callE FVS VS +' E) VS VS 
+    (TR_E (callE FVS VS +' E))
+    (VR_E (callE FVS VS +' E))
+    (fun a1 a2 => @VR_D_DE _ _ (Call (fn, (vs1, st1))) a1
+                               (Call (fn, (vs2, st2))) a2)  
+    (evalE_fun pr1 (fn, (vs1, st1))) (evalE_fun pr2 (fn, (vs2, st2))).
+  intros.
+  unfold evalE_fun; simpl.
+Admitted. 
+*)  
+
+(* ME: relation between FCState events *)
+Definition TR_D_ME {T1 T2} (d1 : FCState T1)
+                           (d2 : FCState T2) : Prop :=
+  match (d1, d2) with
+  | (FLCode c1 st1, FLCode c2 st2) => RC c1 c2 /\ RS st1 st2
+  | (FFCall xs1 fn1 es1 st1, FFCall xs2 fn2 es2 st2) =>
+      xs2 = map tr_lval xs1 /\ fn1 = fn2 /\ es2 = map tr_expr es1 /\ RS st1 st2
+  | _ => False   
+  end.               
+
+(* ME: relation between FCState event outputs, i.e. over estate *)
+Program Definition VR_D_ME {T1 T2}
+  (d1 : FCState T1) (t1: T1) (d2 : FCState T2) (t2: T2) : Prop.
+  remember d1 as D1.
+  remember d2 as D2.
+  dependent destruction d1.
+  - dependent destruction d2.
+    + exact (RS t1 t2).
+    + exact (False).
+  - dependent destruction d2.
+    + exact (False).
+    + exact (RS t1 t2).
+Defined.      
+
+Program Definition TR_DE_ME : prerel (FCState +' E) (FCState +' E) :=
+  sum_prerel (@TR_D_ME) (TR_E E).
+
+Program Definition VR_DE_ME : postrel (FCState +' E) (FCState +' E) :=
+  sum_postrel (@VR_D_ME) (VR_E E).
+
+Context (fcstate_t_def : TR_E (FCState +' E) = TR_DE_ME).
+Context (fcstate_v_def : VR_E (FCState +' E) = VR_DE_ME).
+
+Lemma comp_gen_ok_ME (fn: funname)
+  (xs1 xs2: lvals) (es1 es2: pexprs) (st1 st2: estate) :
+  xs2 = map tr_lval xs1 ->
+  es2 = map tr_expr es1 -> 
+  RS st1 st2 ->
+  @rutt (FCState +' E) _ _ _ (TR_E _) (VR_E _)
+    (fun a1 a2 => @VR_D_ME _ _ (FFCall_ xs1 fn es1 st1) a1
+                             (FFCall_ xs2 fn es2 st2) a2)  
+    (meval_fcall pr1 xs1 fn es1 st1) (meval_fcall pr2 xs2 fn es2 st2).
+  intros.
+  unfold meval_fcall; simpl.
+  
+  eapply rutt_bind with (RR := RV).
+  unfold err_eval_Args.
+  (* OK *)
+  admit.
+
+  intros.
+  eapply rutt_bind with (RR := RS).
+  unfold err_init_state.
+  (* OK *)
+  admit.
+
+  intros.
+  eapply rutt_bind with (RR := RC).
+  unfold err_get_FunCode.
+  (* OK *)
+  admit.
+
+  intros.
+  inv H4.
+  eapply rutt_bind with (RR := RS).
+  eapply rutt_trigger; simpl.
+  rewrite fcstate_t_def.
+  unfold TR_DE_ME.
+  econstructor.
+  unfold TR_D_ME.
+  split; auto.
+
+  intros.
+  (* OK *)
+  admit.
+
+  intros.
+  eapply rutt_bind with (RR := RV).
+  unfold err_return_val.
+  (* OK *)
+  admit.
+
+  intros.
+  unfold err_reinstate_caller.
+  (* OK *)
+  admit.
+Admitted. 
+
+
+
+(* Inductive lemma *)
+Lemma rutt_cmd_tr_ME_step (cc: cmd) (st1 st2: estate) : 
+  RS st1 st2 ->
+  @rutt (FCState +' E) _ _ _
+    (sum_prerel (@TR_D_ME) (TR_E E))
+    (sum_postrel (@VR_D_ME) (VR_E E))
+    RS (st_cmd_map_r (meval_instr pr1) cc st1)
+    (st_cmd_map_r (meval_instr pr2) (Tr_cmd cc) st2).
+  simpl; intros.
+
+  set (Pr := fun (i: instr_r) => forall ii st1 st2, RS st1 st2 -> 
+     @rutt (FCState +' E) _ _ _
+    (sum_prerel (@TR_D_ME) (TR_E E))
+    (sum_postrel (@VR_D_ME) (VR_E E))
+    RS 
+    (st_cmd_map_r (meval_instr pr1) ((MkI ii i) :: nil) st1)
+    (st_cmd_map_r (meval_instr pr2) ((Tr_instr (MkI ii i)) :: nil) st2)).
+
+  set (Pi := fun (i: instr) => forall st1 st2, RS st1 st2 -> 
+     @rutt (FCState +' E) _ _ _
+    (sum_prerel (@TR_D_ME) (TR_E E))
+    (sum_postrel (@VR_D_ME) (VR_E E))
+    RS 
+    (st_cmd_map_r (meval_instr pr1) (i :: nil) st1)
+    (st_cmd_map_r (meval_instr pr2) ((Tr_instr i) :: nil) st2)).
+
+  set (Pc := fun (c: cmd) => forall st1 st2, RS st1 st2 -> 
+     @rutt (FCState +' E) _ _ _
+    (sum_prerel (@TR_D_ME) (TR_E E))
+    (sum_postrel (@VR_D_ME) (VR_E E))
+    RS 
+    (st_cmd_map_r (meval_instr pr1) c st1)
+    (st_cmd_map_r (meval_instr pr2) (Tr_cmd c) st2)).
+
+  revert H.
+  revert st1 st2.
+  revert cc.
+  apply (cmd_Ind Pr Pi Pc); rewrite /Pr /Pi /Pc; simpl; eauto; intros.
+
+  { eapply rutt_Ret; eauto. }
+  { destruct i; simpl.
+    eapply rutt_bind with (RR := RS); simpl in *.
+
+    specialize (H st1 st2 H1).
+    (* PROBLEM: we need to invert H. probably need a coinductive proof *)
+    admit.
+
+    intros; auto.
+  }
+
+  { eapply rutt_bind with (RR := RS).
+    unfold ret_mk_AssgnE.
+    (* OK admit *)
+    admit.
+
+    intros.
+    eapply rutt_Ret; eauto.
+  }
+
+  { eapply rutt_bind with (RR := RS).
+    (* OK admit *)
+    admit.
+
+    intros.
+    eapply rutt_Ret; eauto.
+  }
+
+  { eapply rutt_bind with (RR := RS).
+    (* OK admit *)
+    admit.
+
+    intros.
+    eapply rutt_Ret; eauto.
+  }
+
+  { intros.
+    eapply rutt_bind with (RR := RS).
+    eapply rutt_bind with (RR := eq).
+    
+    unfold err_mk_EvalCond.
+    (* OK *)
+    admit.
+
+    intros.
+    inv H2; simpl.
+    destruct r2; simpl.
+
+    eapply H; eauto.
+    eapply H0; eauto.
+
+    intros.
+    eapply rutt_Ret; auto.
+  }
+
+  { eapply rutt_bind with (RR := RS); simpl.
+    destruct rn.
+    destruct p; simpl.    
+    eapply rutt_bind with (RR := eq); simpl.
+    unfold err_mk_EvalBound; simpl.
+    (* OK *)
+    admit.
+
+    intros.
+    inv H1.
+    eapply rutt_bind with (RR := eq); simpl.
+    unfold err_mk_EvalBound; simpl.
+    (* OK *)
+    admit.
+
+    intros.
+    inv H1.
+
+    revert H0.
+    revert st1 st2.
+    induction (wrange d r2 r0); simpl; intros.
+    { eapply rutt_Ret; eauto. }
+    { eapply rutt_bind with (RR:= RS); simpl.
+      (* OK *)
+      admit.
+
+      intros.
+      eapply rutt_bind with (RR := RS).
+      eapply H; eauto.
+      intros; auto.
+    }
+      
+    intros.
+    eapply rutt_Ret; auto.
+  }
+    
+  { eapply rutt_bind with (RR := RS).
+    eapply rutt_iter with (RI := RS); auto.
+    intros.
+    eapply rutt_bind with (RR := RS).
+    eapply H; auto.
+
+    intros.
+    eapply rutt_bind with (RR := eq).
+    (* OK *)
+    admit.
+
+    intros.
+    inv H4.
+    destruct r3.
+
+    eapply rutt_bind with (RR := RS); auto.
+    intros.
+    eapply rutt_Ret; auto.
+    eapply rutt_Ret; auto.
+
+    intros.
+    eapply rutt_Ret; auto.
+  }   
+    
+  { eapply rutt_bind with (RR := RS).
+    eapply rutt_trigger; simpl.
+    econstructor.
+    unfold TR_D_ME; simpl.
+    split; eauto.
+
+    intros; auto.
+    (* OK *)
+    admit.
+
+    intros; auto.
+    eapply rutt_Ret; auto.
+  }  
+Admitted.     
+  
+(* Here we apply the inductive lemma and comp_gen_ok *)
+Lemma rutt_cmd_tr_ME (cc: cmd) (st1 st2: estate) : 
+  RS st1 st2 ->
+  @rutt E _ _ _ 
+    (TR_E _) (VR_E _) RS
+    (mevalE_cmd pr1 cc st1) (mevalE_cmd pr2 (Tr_cmd cc) st2).
+  intros.
+  unfold mevalE_cmd; simpl.
+  eapply interp_mrec_rutt.
+  intros.
+  instantiate (3 := @TR_D_ME).
+  instantiate (1 := @VR_D_ME).
+  unfold meval_cstate.
+  destruct d1.
+  unfold TR_D_ME in H0.
+  destruct d2; try intuition.
+  inv H1; simpl.
+  eapply rutt_cmd_tr_ME_step; eauto. 
+   
+  unfold TR_D_ME in H0.
+  destruct d2; simpl in *; try intuition.
+  inv H0.  
+  set CC := (comp_gen_ok_ME f0 xs _ es _ _ _ erefl erefl H4).
+  setoid_rewrite fcstate_t_def in CC.
+  setoid_rewrite fcstate_v_def in CC.
+  exact CC.
+    
+  simpl.
+  eapply rutt_cmd_tr_ME_step; eauto. 
+Qed.   
+
+End Sample_proof.
+
+
+
+Section Const_prop.
+
+Context (pr1 : prog).
+Context (gd: glob_decls).
+
+Context (globs: globals).
+
+Local Notation cpm := (Mvar.t const_v).
+
+Variable const_prop_i : cpm -> instr -> cpm * cmd.
+
+Let pr2 := const_prop_prog pr1.
+
+Context (E: Type -> Type).   
+Context (HasErr: ErrState -< E).   
+
+Local Notation RS := (@eq estate).
+Local Notation RV1 := (value_uincl).
+Local Notation RV := (List.Forall2 value_uincl).
+
+Local Notation VS := (values * estate)%type.
+Local Notation FVS := (funname * VS)%type.
+
+Notation RVS := (fun (vs_st1 vs_st2 : VS) => 
+  (RV vs_st1.1 vs_st2.1 /\ RS vs_st1.2 vs_st2.2)).
+Notation RFVS := (fun (fvs1 fvs2 : FVS) => 
+  (fvs1.1 = fvs2.1 /\ RVS fvs1.2 fvs2.2)).
+
+Notation RC' := (fun (c1 c2: cmd) (g1 g2: cpm) =>
+                  (g2, c2) = const_prop g1 c1).
+Notation RC := (fun (c1 c2: cmd) => exists (g1 g2: cpm),
+                  (g2, c2) = const_prop g1 c1).
+
+Context (TR_E : forall T1 T2,
+            E T1 -> E T2 -> Prop)
+        (VR_E : forall T1 T2,
+            E T1 -> T1 -> E T2 -> T2 -> Prop).
+
+
+(* ME: relation between FCState events *)
+Definition TR_D_ME' {T1 T2} (d1 : FCState T1)
+                            (d2 : FCState T2) : Prop :=
+  match (d1, d2) with
+  | (FLCode c1 st1, FLCode c2 st2) => (forall g1: cpm, exists g2: cpm,
+                  (g2, c2) = const_prop const_prop_i g1 c1) /\ RS st1 st2
+  | (FFCall xs1 fn1 es1 st1, FFCall xs2 fn2 es2 st2) =>
+      xs2 = map tr_lval xs1 /\ fn1 = fn2
+      /\ (forall g1: cpm, es2 = map (const_prop_e globs g1) es1) /\ RS st1 st2
+  | _ => False   
+  end.               
+
+(* ME: relation between FCState event outputs, i.e. over estate *)
+Program Definition VR_D_ME' {T1 T2}
+  (d1 : FCState T1) (t1: T1) (d2 : FCState T2) (t2: T2) : Prop.
+  remember d1 as D1.
+  remember d2 as D2.
+  dependent destruction d1.
+  - dependent destruction d2.
+    + exact (RS t1 t2).
+    + exact (False).
+  - dependent destruction d2.
+    + exact (False).
+    + exact (RS t1 t2).
+Defined.      
+
+(*
+Check @sum_prerel.
+About prerel.
+Print HeterogeneousRelations.prerel.
+Check @sum_prerel.
+*)
+
+Program Definition TR_DE_ME' : prerel (FCState +' E) (FCState +' E) :=
+  sum_prerel (@TR_D_ME') TR_E.
+
+Program Definition VR_DE_ME' : postrel (FCState +' E) (FCState +' E) :=
+  sum_postrel (@VR_D_ME') VR_E.
+
+(*
+Context (fcstate_t_def : TR_E (FCState +' E) = TR_DE_ME).
+Context (fcstate_v_def : VR_E (FCState +' E) = VR_DE_ME).
+*)
+
+Lemma constant_prop_ME (fn: funname)
+  (xs1 xs2: lvals) (es1 es2: pexprs) (st1 st2: estate) :
+  xs2 = map tr_lval xs1 ->
+  es2 = map tr_expr es1 -> 
+  RS st1 st2 ->
+  @rutt (FCState +' E) (FCState +' E) estate estate TR_DE_ME' VR_DE_ME'
+    (fun a1 a2 => @VR_D_ME' _ _ (FFCall_ xs1 fn es1 st1) a1
+                                (FFCall_ xs2 fn es2 st2) a2)  
+    (meval_fcall pr1 xs1 fn es1 st1) (meval_fcall pr2 xs2 fn es2 st2).
+  intros.
+  unfold meval_fcall; simpl.
+  
+  eapply rutt_bind with (RR := RV).
+  unfold err_eval_Args.
+  (* OK *)
+  admit.
+
+  intros.
+  eapply rutt_bind with (RR := RS).
+  unfold err_init_state.
+  (* OK *)
+  admit.
+
+  intros.
+  eapply rutt_bind with (RR := RC).
+  unfold err_get_FunCode.
+  (* OK *)
+  admit.
+
+  intros.
+  inv H4.
+  eapply rutt_bind with (RR := RS).
+  eapply rutt_trigger; simpl.
+  rewrite fcstate_t_def.
+  unfold TR_DE_ME.
+  econstructor.
+  unfold TR_D_ME.
+  split; auto.
+
+  intros.
+  (* OK *)
+  admit.
+
+  intros.
+  eapply rutt_bind with (RR := RV).
+  unfold err_return_val.
+  (* OK *)
+  admit.
+
+  intros.
+  unfold err_reinstate_caller.
+  (* OK *)
+  admit.
+Admitted. 
+
+
+
+(* Inductive lemma *)
+Lemma rutt_cmd_tr_ME_step (cc: cmd) (st1 st2: estate) : 
+  RS st1 st2 ->
+  @rutt (FCState +' E) _ _ _
+    (sum_prerel (@TR_D_ME) (TR_E E))
+    (sum_postrel (@VR_D_ME) (VR_E E))
+    RS (st_cmd_map_r (meval_instr pr1) cc st1)
+    (st_cmd_map_r (meval_instr pr2) (Tr_cmd cc) st2).
+  simpl; intros.
+
+  set (Pr := fun (i: instr_r) => forall ii st1 st2, RS st1 st2 -> 
+     @rutt (FCState +' E) _ _ _
+    (sum_prerel (@TR_D_ME) (TR_E E))
+    (sum_postrel (@VR_D_ME) (VR_E E))
+    RS 
+    (st_cmd_map_r (meval_instr pr1) ((MkI ii i) :: nil) st1)
+    (st_cmd_map_r (meval_instr pr2) ((Tr_instr (MkI ii i)) :: nil) st2)).
+
+  set (Pi := fun (i: instr) => forall st1 st2, RS st1 st2 -> 
+     @rutt (FCState +' E) _ _ _
+    (sum_prerel (@TR_D_ME) (TR_E E))
+    (sum_postrel (@VR_D_ME) (VR_E E))
+    RS 
+    (st_cmd_map_r (meval_instr pr1) (i :: nil) st1)
+    (st_cmd_map_r (meval_instr pr2) ((Tr_instr i) :: nil) st2)).
+
+  set (Pc := fun (c: cmd) => forall st1 st2, RS st1 st2 -> 
+     @rutt (FCState +' E) _ _ _
+    (sum_prerel (@TR_D_ME) (TR_E E))
+    (sum_postrel (@VR_D_ME) (VR_E E))
+    RS 
+    (st_cmd_map_r (meval_instr pr1) c st1)
+    (st_cmd_map_r (meval_instr pr2) (Tr_cmd c) st2)).
+
+  revert H.
+  revert st1 st2.
+  revert cc.
+  apply (cmd_Ind Pr Pi Pc); rewrite /Pr /Pi /Pc; simpl; eauto; intros.
+
+  { eapply rutt_Ret; eauto. }
+  { destruct i; simpl.
+    eapply rutt_bind with (RR := RS); simpl in *.
+
+    specialize (H st1 st2 H1).
+    (* PROBLEM: we need to invert H. probably need a coinductive proof *)
+    admit.
+
+    intros; auto.
+  }
+
+  { eapply rutt_bind with (RR := RS).
+    unfold ret_mk_AssgnE.
+    (* OK admit *)
+    admit.
+
+    intros.
+    eapply rutt_Ret; eauto.
+  }
+
+  { eapply rutt_bind with (RR := RS).
+    (* OK admit *)
+    admit.
+
+    intros.
+    eapply rutt_Ret; eauto.
+  }
+
+  { eapply rutt_bind with (RR := RS).
+    (* OK admit *)
+    admit.
+
+    intros.
+    eapply rutt_Ret; eauto.
+  }
+
+  { intros.
+    eapply rutt_bind with (RR := RS).
+    eapply rutt_bind with (RR := eq).
+    
+    unfold err_mk_EvalCond.
+    (* OK *)
+    admit.
+
+    intros.
+    inv H2; simpl.
+    destruct r2; simpl.
+
+    eapply H; eauto.
+    eapply H0; eauto.
+
+    intros.
+    eapply rutt_Ret; auto.
+  }
+
+  { eapply rutt_bind with (RR := RS); simpl.
+    destruct rn.
+    destruct p; simpl.    
+    eapply rutt_bind with (RR := eq); simpl.
+    unfold err_mk_EvalBound; simpl.
+    (* OK *)
+    admit.
+
+    intros.
+    inv H1.
+    eapply rutt_bind with (RR := eq); simpl.
+    unfold err_mk_EvalBound; simpl.
+    (* OK *)
+    admit.
+
+    intros.
+    inv H1.
+
+    revert H0.
+    revert st1 st2.
+    induction (wrange d r2 r0); simpl; intros.
+    { eapply rutt_Ret; eauto. }
+    { eapply rutt_bind with (RR:= RS); simpl.
+      (* OK *)
+      admit.
+
+      intros.
+      eapply rutt_bind with (RR := RS).
+      eapply H; eauto.
+      intros; auto.
+    }
+      
+    intros.
+    eapply rutt_Ret; auto.
+  }
+    
+  { eapply rutt_bind with (RR := RS).
+    eapply rutt_iter with (RI := RS); auto.
+    intros.
+    eapply rutt_bind with (RR := RS).
+    eapply H; auto.
+
+    intros.
+    eapply rutt_bind with (RR := eq).
+    (* OK *)
+    admit.
+
+    intros.
+    inv H4.
+    destruct r3.
+
+    eapply rutt_bind with (RR := RS); auto.
+    intros.
+    eapply rutt_Ret; auto.
+    eapply rutt_Ret; auto.
+
+    intros.
+    eapply rutt_Ret; auto.
+  }   
+    
+  { eapply rutt_bind with (RR := RS).
+    eapply rutt_trigger; simpl.
+    econstructor.
+    unfold TR_D_ME; simpl.
+    split; eauto.
+
+    intros; auto.
+    (* OK *)
+    admit.
+
+    intros; auto.
+    eapply rutt_Ret; auto.
+  }  
+Admitted.     
+  
+(* Here we apply the inductive lemma and comp_gen_ok *)
+Lemma rutt_cmd_tr_ME (cc: cmd) (st1 st2: estate) : 
+  RS st1 st2 ->
+  @rutt E _ _ _ 
+    (TR_E _) (VR_E _) RS
+    (mevalE_cmd pr1 cc st1) (mevalE_cmd pr2 (Tr_cmd cc) st2).
+  intros.
+  unfold mevalE_cmd; simpl.
+  eapply interp_mrec_rutt.
+  intros.
+  instantiate (3 := @TR_D_ME).
+  instantiate (1 := @VR_D_ME).
+  unfold meval_cstate.
+  destruct d1.
+  unfold TR_D_ME in H0.
+  destruct d2; try intuition.
+  inv H1; simpl.
+  eapply rutt_cmd_tr_ME_step; eauto. 
+   
+  unfold TR_D_ME in H0.
+  destruct d2; simpl in *; try intuition.
+  inv H0.  
+  set CC := (comp_gen_ok_ME f0 xs _ es _ _ _ erefl erefl H4).
+  setoid_rewrite fcstate_t_def in CC.
+  setoid_rewrite fcstate_v_def in CC.
+  exact CC.
+    
+  simpl.
+  eapply rutt_cmd_tr_ME_step; eauto. 
+Qed.   
+
+End Const_prop.
+
+
+
+
+
+End TRANSF.
+
+End WSW.
+
+End Lang.
+
+
